cslib/Cslib/Languages/LambdaCalculus/LocallyNameless/Untyped/FullBetaEtaConfluence.lean
@@ -88,7 +88,7 @@ lemma stronglyCommute_eta_beta : StronglyCommute (@FullEta Var) FullBeta := by
         | refl => grind [open_close]
         | single => exact .single (Xi.abs {w} (by grind [FullBeta.redex_subst_cong]))
       · rw [open_close w N 0 (by grind)]
-        exact FullEta.redex_abs_close h_eta (FullBeta.step_lc_r (st_body_beta w (by grind)))
+        exact FullEta.redex_abs_close h_eta
 
 open Commute in
 /-- βη-reduction is confluent. -/
